L20/Expr.v
@@ -7,6 +7,16 @@ From Vyper.L10 Require Import Base.
 From Vyper.L20 Require Import AST Callset Descend.
 
 
+Definition storage_var_is_declared {C: VyperConfig}
+                                   (cd: calldag)
+                                   (name: string)
+: bool
+:= match cd_declmap cd name with
+   | Some (StorageVarDecl _) => true
+   | _ => false
+   end.
+
+
 Fixpoint interpret_expr {C: VyperConfig}
                         {bigger_call_depth_bound smaller_call_depth_bound: nat}
                         (Ebound: bigger_call_depth_bound = S smaller_call_depth_bound)
@@ -58,13 +68,15 @@ Fixpoint interpret_expr {C: VyperConfig}
        | LocalVar name => fun _ =>
            (world, match map_lookup loc name with
                    | Some val => ExprSuccess val
-                   | None => expr_error "Local variable not found"
+                   | None => expr_error "undeclared local variable"
                    end)
-       | StorageVar name => fun _ => 
-           (world, match storage_lookup world name with
-                   | Some val => ExprSuccess val
-                   | None => expr_error "Storage variable not found"
-                   end)
+       | StorageVar name => fun _ =>
+           if storage_var_is_declared cd name
+              then (world, ExprSuccess (match storage_lookup world name with
+                                        | None => zero256
+                                        | Some x => x
+                                        end))
+              else (world, expr_error "undeclared global variable")
        | UnOp op a => fun E =>
            let (world', result) := interpret_expr Ebound fc do_call builtins
                                                   world loc a
