From10To20/Stmt.v
@@ -1,0 +1,223 @@
+From Coq Require Import String ZArith Eqdep_dec.
+
+From Coq Require PropExtensionality.
+
+From Vyper Require Import Config Calldag L10.Base.
+From Vyper Require L10.AST L10.Expr L20.AST L10.Interpret L20.Interpret.
+
+From Vyper.From10To20 Require Import Translate Callset FunCtx Expr.
+
+(* This tactic applies interpret_translated_expr wherever possible. *)
+Local Ltac expr :=
+  let e20 := fresh "e20" in
+  let e10 := fresh "e10" in
+  let E := fresh "E" in
+  remember (L20.Expr.interpret_expr _ _ _ _ _ _ _ _) as e20;
+  remember (L10.Expr.interpret_expr _ _ _ _ _ _ _ _) as e10;
+  assert (E: e20 = e10) by (subst; now apply interpret_translated_expr);
+  rewrite E; clear E; subst e10; subst e20.
+
+
+Lemma interpret_translated_small_stmt {C: VyperConfig}
+                                {bigger_call_depth_bound smaller_call_depth_bound: nat}
+                                (Ebound: bigger_call_depth_bound = S smaller_call_depth_bound)
+                                {cd: L10.Descend.calldag}
+                                (builtins: string -> option builtin)
+                                (fc: fun_ctx cd bigger_call_depth_bound)
+                                {cd2: L20.Descend.calldag}
+                                (ok: cd2 = translate_calldag cd)
+                                {do_call_10: forall
+                                      (fc': fun_ctx cd smaller_call_depth_bound)
+                                      (world: world_state)
+                                      (arg_values: list uint256),
+                                    world_state * expr_result uint256}
+                                {do_call_20: forall
+                                      (fc': fun_ctx cd2 smaller_call_depth_bound)
+                                      (world: world_state)
+                                      (arg_values: list uint256),
+                                    world_state * expr_result uint256}
+                                (DoCallOk: forall fc' world arg_values,
+                                             do_call_20 (translate_fun_ctx fc' ok) world arg_values
+                                              =
+                                             do_call_10 fc' world arg_values)
+                                (world: world_state)
+                                (loc: string_map uint256)
+                                {ss10: L10.AST.small_stmt}
+                                {s20: L20.AST.stmt}
+                                (StmtOk: s20 = let is_private_call := fun name: string =>
+                                                  match cd_declmap cd name with
+                                                  | Some _ => true
+                                                  | _ => false
+                                                  end
+                                               in translate_small_stmt is_private_call ss10)
+                                (CallOk20: let _ := string_set_impl in 
+                                   FSet.is_subset (L20.Callset.stmt_callset s20)
+                                                  (L20.Callset.decl_callset
+                                                     (fun_decl
+                                                       (translate_fun_ctx fc ok)))
+                                   = true)
+                                (CallOk10: let _ := string_set_impl in 
+                                   FSet.is_subset (L10.Callset.small_stmt_callset ss10)
+                                                  (L10.Callset.decl_callset
+                                                    (fun_decl fc))
+                                   = true):
+   L20.Stmt.interpret_stmt Ebound (translate_fun_ctx fc ok) do_call_20 builtins
+                           world loc s20 CallOk20
+    =
+   L10.Stmt.interpret_small_stmt Ebound fc do_call_10 builtins
+                                 world loc ss10 CallOk10.
+Proof.
+induction ss10.
+{ (* pass *) now subst. }
+{ (* break *) now subst. }
+{ (* continue *) now subst. }
+{ (* return *)
+  subst. cbn.
+  destruct result. 2:{ easy. }
+  cbn. now expr.
+}
+{ (* revert *) now subst. }
+{ (* raise *)
+  subst. cbn. expr.
+  now L10.Expr.destruct_let_pair.
+}
+{ (* assert *)
+  subst. cbn. expr.
+  L10.Expr.destruct_let_pair.
+  destruct e. 2:{ trivial. }
+  destruct ((Z_of_uint256 value =? 0)%Z). 2:{ trivial. }
+  destruct error. 2: { easy. }
+  (* there's an error message *)
+  expr.
+  L10.Expr.destruct_let_pair.
+  match goal with
+  |- _ = match ?e with | ExprSuccess _ => _ | ExprAbort _ => _ end => now destruct e
+  end.
+}
+{ (* assign *)
+  subst. cbn. expr.
+  L10.Expr.destruct_let_pair.
+  unfold L10.Stmt.do_assign. unfold L20.Stmt.do_assign.
+  destruct e. 2:{ trivial. } 
+  destruct lhs. { trivial. }
+  now rewrite storage_var_is_declared_ok.
+}
+{ (* binop assign *)
+  subst. cbn.
+  destruct lhs; cbn.
+  { (* local var *)
+    unfold map_lookup.
+    remember (Map.lookup loc name) as m.
+    destruct m.
+    {
+      expr.
+      destruct L10.Expr.interpret_expr.
+      unfold L20.Stmt.do_assign.
+      destruct e. 2:{ trivial. }
+      rewrite<- Heqm. trivial.
+    }
+    unfold expr_error. trivial.
+  }
+  (* global var *)
+  rewrite storage_var_is_declared_ok.
+  unfold L20.Stmt.do_assign.
+  remember (L10.Expr.storage_var_is_declared _ _) as is_declared.
+  destruct is_declared. 2:easy.
+  expr.
+  destruct L10.Expr.interpret_expr.
+  destruct e. 2:{ trivial. }
+  rewrite storage_var_is_declared_ok.
+  rewrite<- Heqis_declared.
+  trivial.
+}
+(* expr *)
+subst. cbn. expr.
+now L10.Expr.destruct_let_pair.
+Qed.
+
+(*
+
+
+
+Theorem interpret_translated_call {C: VyperConfig}
+                                  (builtins: string -> option L10.Interpret.builtin)
+                                  {cd: L10.Interpret.calldag}
+                                  {call_depth_bound: nat}
+                                  (fc: L10.Interpret.fun_ctx cd call_depth_bound)
+                                  {cd2: L20.Interpret.calldag}
+                                  (ok: cd2 = translate_calldag cd)
+                                  (world: world_state)
+                                  (arg_values: list uint256):
+  L20.Interpret.interpret_call builtins (translate_fun_ctx fc ok) world arg_values
+   =
+  L10.Interpret.interpret_call builtins fc world arg_values.
+Proof.
+induction call_depth_bound.
+{ exfalso. exact (Nat.nlt_0_r _ (L10.Interpret.fun_bound_ok _ _ fc)). }
+pose (is_private_call := fun name: string =>
+          match L10.Interpret.cd_declmap _ _ cd name with
+          | Some _ => true
+          | _ => false
+          end).
+assert(F: L20.Interpret.fun_decl _ _ (translate_fun_ctx fc ok)
+           = 
+          translate_decl is_private_call (L10.Interpret.fun_decl _ _ fc)).
+{
+  clear IHcall_depth_bound.
+  unfold translate_fun_ctx in *. cbn in *.
+  unfold cached_translated_decl in *.
+  remember (translate_fun_ctx_fun_decl_helper fc ok) as foo. clear Heqfoo.
+  remember (Interpret.cd_declmap cd2 (L10.Interpret.fun_name cd (S call_depth_bound) fc)) as d.
+  destruct d. 2:{ contradiction. }
+  subst. cbn in Heqd.
+  remember (L10.Interpret.cd_declmap L10.AST.decl L10.Callset.decl_callset cd
+                                     (L10.Interpret.fun_name cd (S call_depth_bound) fc)) as x.
+  destruct x. 2:{ discriminate. }
+  inversion Heqd. unfold is_private_call.
+  f_equal. inversion Heqx.
+  assert (D := L10.Interpret.fun_decl_ok _ _ fc).
+  rewrite D in *. inversion H1. (* XXX *)
+  trivial.
+}
+unfold L20.Interpret.interpret_call.
+unfold L10.Interpret.interpret_call.
+rewrite F.
+
+
+
+
+
+
+  intro H. clear H.
+  
+  
+  
+remember  as d10.
+
+
+unfold translate_fun_ctx. unfold cached_translated_decl.
+remember (L10.Interpret.fun_name _ _ fc) as fun_name.
+
+unfold translate_fun_ctx.
+
+
+
+
+
+Theorem translate_ok {C: VyperConfig}
+                     (builtins: string -> option L10.Interpret.builtin)
+                     (cd: L10.Interpret.calldag)
+                     (fun_name: string)
+                     (world: world_state)
+                     (arg_values: list uint256):
+  L20.Interpret.interpret builtins (translate_calldag cd) fun_name world arg_values
+   =
+  L10.Interpret.interpret builtins cd fun_name world arg_values.
+Proof.
+unfold L10.Interpret.interpret. unfold L20.Interpret.interpret.
+remember (L10.Interpret.cd_declmap cd fun_name) as d. 
+unfold translate_calldag.
+unfold L20.Interpret.make_fun_ctx_and_bound. cbn.
+revert translate_dag_helper.
+destruct d.
+*)
